veric/initialize.v
@@ -164,63 +164,6 @@ Proof.
 Qed.
 
 
-Lemma alloc_globals_app:
-   forall F V (ge: Genv.t F V) m m2 vs vs',
-  Genv.alloc_globals ge m (vs++vs') = Some m2 <->
-    exists m', Genv.alloc_globals ge m vs = Some m' /\
-                    Genv.alloc_globals ge m' vs' = Some m2.
-Proof.
-intros.
-revert vs' m m2; induction vs; intros.
-simpl.
-intuition. exists m; intuition. destruct H as [? [H ?]]; inv H; auto.
-simpl.
-case_eq (Genv.alloc_global ge m a); intros.
-specialize (IHvs vs' m0 m2).
-auto.
-intuition; try discriminate.
-destruct H0 as [? [? ?]]; discriminate.
-Qed.
-
-Fixpoint alloc_globals_rev {F V} (ge: Genv.t F V) (m: mem) (vl: list (ident * globdef F V))
-                         {struct vl} : option mem :=
-  match vl with
-  | nil => Some m
-  | v :: vl' =>
-     match alloc_globals_rev ge m vl' with
-     | Some m' => Genv.alloc_global ge m' v
-     | None => None
-     end
-  end.
-
-Lemma alloc_globals_rev_eq: 
-     forall F V (ge: Genv.t F V) m vl,
-     Genv.alloc_globals ge m (rev vl) = alloc_globals_rev ge m vl.
-Proof.
-intros.
-revert m; induction vl; intros; auto.
-simpl.
-rewrite <- IHvl.
-case_eq (Genv.alloc_globals ge m (rev vl)); intros.
-case_eq (Genv.alloc_global ge m0 a); intros.
-rewrite alloc_globals_app.
-exists m0; split; auto.
-simpl. rewrite H0; auto.
-case_eq (Genv.alloc_globals ge m (rev vl ++ a :: nil)); intros; auto.
-elimtype False.
-apply alloc_globals_app in H1.
-destruct H1 as [m' [? ?]].
-inversion2 H H1.
-simpl in H2.
-rewrite H0 in H2; inv H2.
-case_eq (Genv.alloc_globals ge m (rev vl ++ a :: nil)); intros; auto.
-elimtype False.
-apply alloc_globals_app in H0.
-destruct H0 as [m' [? ?]].
-inversion2 H H0.
-Qed.
-
-
 Lemma rev_prog_vars': forall {F V} vl, rev (@prog_vars' F V vl) = prog_vars' (rev vl).
 Proof.
    intros.
@@ -830,18 +773,6 @@ Proof.
   apply H2.
 Qed.
 
-Lemma store_zeros_access:  forall m b z N m',
-      Genv.store_zeros m b z N = Some m' -> access_at m' = access_at m.
-Proof.
- intros. symmetry in H; apply Genv.R_store_zeros_correct in H.
- remember (Some m') as m1. revert m' Heqm1; induction H; intros; inv Heqm1.
- auto.
- rewrite (IHR_store_zeros m'0 (eq_refl _)).
- clear - e0.
- Transparent store. unfold store in e0.
- if_tac in e0; inv e0. unfold access_at; simpl. auto.
-Qed.
-
 Lemma init_data_list_size_app:
   forall dl1 dl2, Genv.init_data_list_size (dl1++dl2) = 
                    Genv.init_data_list_size dl1 + Genv.init_data_list_size dl2.
@@ -1050,20 +981,6 @@ Proof. induction vl; simpl; auto.
   rewrite <- andb_assoc. f_equal; auto.
 Qed.
 
-Lemma store_zeros_contents1: forall m b z N m' loc,
-      fst loc <> b ->
-      Genv.store_zeros m b z N = Some m' -> 
-      contents_at m loc = contents_at m' loc.
-Proof.
- intros. symmetry in H0; apply Genv.R_store_zeros_correct in H0.
- remember (Some m') as m1. revert m' Heqm1; induction H0; intros; inv Heqm1.
- auto.
- transitivity (contents_at m' loc). 
- Transparent store. unfold store in e0.
- if_tac in e0; inv e0. unfold contents_at; simpl. rewrite ZMap.gso by auto. auto.
- eapply IHR_store_zeros; eauto.
-Qed.
-
 Lemma store_init_data_list_access:
   forall  {F V} (ge: Genv.t F V) m b z dl m', 
      Genv.store_init_data_list ge m b z dl = Some m' -> 
@@ -1103,65 +1020,6 @@ Proof.
     f_equal; auto. auto.
 Qed.
 
-
-Lemma nth_error_app: forall {T} (al bl : list T) (j: nat),
-     nth_error (al++bl) (length al + j) = nth_error bl j.
-Proof.
- intros. induction al; simpl; auto.
-Qed.
-Lemma nth_error_app1: forall {T} (al bl : list T) (j: nat),
-     (j < length al)%nat ->
-     nth_error (al++bl) j = nth_error al j.
-Proof.
-  intros. revert al H; induction j; destruct al; simpl; intros; auto; try omegaContradiction.
-   apply IHj. omega.
-Qed.
-
-Lemma alloc_global_old:
-  forall {F V} (ge: Genv.t F V) m iv m', Genv.alloc_global ge m iv = Some m' ->
-       forall loc, fst loc < nextblock m ->
-        access_at m loc = access_at m' loc /\ contents_at m loc = contents_at m' loc.
-Proof.
- intros.
- destruct loc as [b ofs]; simpl in *; subst.
- assert (NEQ: b <> nextblock m) by (intro Hx; inv Hx; omega).
- unfold Genv.alloc_global in H. destruct iv.
- destruct g.
- revert H; case_eq (alloc m 0 1); intros.
- unfold drop_perm in H1. 
- destruct (range_perm_dec m0 b0 0 1 Cur Freeable); inv H1.
- unfold contents_at, access_at in *; 
- simpl in *.
- Transparent alloc. unfold alloc in H. Opaque alloc.
- inv H; simpl in *.
- rewrite ZMap.gss. repeat rewrite (ZMap.gso _ _ NEQ). auto.
-
- forget (Genv.init_data_list_size (gvar_init v)) as N.
- revert H; case_eq (alloc m 0 N); intros.
- invSome. invSome.
-  Transparent alloc. unfold alloc in H. Opaque alloc.
-  assert (access_at m (b,ofs) = access_at m0 (b,ofs) /\ contents_at m (b,ofs) = contents_at m0 (b,ofs)).
- clear - H NEQ.
- inv H; 
- unfold contents_at, access_at in *; 
- simpl in *.
- repeat rewrite (ZMap.gso _ _ NEQ). auto.
- assert (b0=nextblock m) by (inv H; auto). subst b0.
- destruct H2  as [H2a H2c]; rewrite H2a; rewrite H2c; clear H H2a H2c.
- rewrite <- (store_zeros_access _ _ _ _ _ H1).
- apply store_zeros_contents1 with (loc:= (b,ofs)) in H1.
- 2: simpl; congruence. rewrite H1; clear H1 m0.
- apply store_init_data_list_outside' in H4.
- destruct H4 as [? [? ?]].
- specialize (H b ofs).  destruct H.
- destruct H; subst; congruence. unfold block in *; rewrite H; rewrite H1.
- clear - H5 NEQ.
- unfold drop_perm in H5.
- destruct (range_perm_dec m2 (nextblock m) 0 N Cur Freeable); inv H5.
- unfold contents_at, access_at in *; 
- simpl in *.
-  repeat rewrite (ZMap.gso _ _ NEQ). auto.
-Qed.
 
 Lemma alloc_global_beyond2:
   forall {F V} (ge: Genv.t F V) m iv m', Genv.alloc_global ge m iv = Some m' ->
@@ -1235,7 +1093,7 @@ Proof.
  unfold inflate_initial_mem.
  repeat rewrite resource_at_make_rmap.
  if_tac.
-  destruct (alloc_global_old _ _ _ _ H _ H1);
+ destruct (alloc_global_old _ _ _ _ H _ H1) as [? [_ ?]];
  unfold inflate_initial_mem'; rewrite H2; rewrite H3; auto.
  destruct (eq_dec (fst loc) (nextblock m0)).
 Focus 2.
@@ -1277,78 +1135,6 @@ rewrite In_rev in H2. rewrite <- map_rev in H2.
  destruct a; simpl in *. if_tac; auto.
 Qed.
 
-Lemma Zlength_app: forall T (al bl: list T),
-    Zlength (al++bl) = Zlength al + Zlength bl.
-Proof. induction al; intros. simpl app; rewrite Zlength_nil; omega.
- simpl app; repeat rewrite Zlength_cons; rewrite IHal; omega.
-Qed.
-Lemma Zlength_rev: forall T (vl: list T), Zlength (rev vl) = Zlength vl.
-Proof. induction vl; simpl; auto. rewrite Zlength_cons. rewrite <- IHvl.
-rewrite Zlength_app. rewrite Zlength_cons. rewrite Zlength_nil; omega.
-Qed.
-
-Lemma Zlength_map: forall A B (f: A -> B) l, Zlength (map f l) = Zlength l.
-Proof. induction l; simpl; auto. repeat rewrite Zlength_cons. f_equal; auto.
-Qed.
-
-Lemma alloc_globals_rev_nextblock:
-  forall {F V} (ge: Genv.t F V) vl m, alloc_globals_rev ge empty vl = Some m ->
-     nextblock m = Zsucc (Zlength vl).
-Proof. 
-  intros.
-   revert m H; induction vl; simpl; intros. inv H; apply nextblock_empty.
-  invSome. apply IHvl in H.
-  apply Genv.alloc_global_nextblock in H2.  rewrite Zlength_cons. rewrite H2.
-  rewrite H. auto.
-Qed.
-
-Lemma find_symbol_add_globals:
-  forall {F V} i g id dl, ~ In i (map fst dl) -> list_norepet (map fst dl) ->
-   (Genv.find_symbol
-      (Genv.add_globals (Genv.empty_genv F V) (dl ++ (i, g) :: nil)) id =
-          Some (1 + Zlength dl) <-> i = id).
-Proof.
-intros.
-  assert (Genv.genv_next (Genv.empty_genv F V) = 1)  by reflexivity.
-  assert (Genv.find_symbol (Genv.empty_genv F V)  id = None) by (intros; apply PTree.gempty).
- forget (Genv.empty_genv F V) as ge. forget 1 as n. 
-  revert ge n H H0 H1 H2; induction dl; intros.
-        simpl. rewrite Zlength_nil.
-        unfold Genv.find_symbol, Genv.add_global in *; simpl.
-        destruct (eq_dec i id); subst. rewrite PTree.gss.         intuition.
-        rewrite PTree.gso by auto. rewrite H2.  split; intro Hx; inv Hx; congruence.
-        simpl; auto.
-        rewrite Zlength_cons. 
-        replace (n + Zsucc (Zlength dl)) with (Zsucc n + Zlength dl) by omega.
-        simpl. simpl in H0. inv H0.
-         simpl in H.
-         destruct a as [a ag]; simpl in *.
-          assert (a<>i /\ ~ In i (map fst dl)) by (clear - H; intuition). clear H; destruct H0.
-         destruct (eq_dec id a).
-         subst id.
-         split; intro; try congruence. elimtype False.
-         clear IHdl.
-        assert (~In a (map fst ((dl++(i,g)::nil)))).
-            rewrite map_app. rewrite in_app_iff.
-          intros [?|?]; try contradiction. simpl in H3. destruct H3; try congruence.
-         forget   (dl ++ (i, g) :: nil) as vl.
-         assert (Genv.find_symbol (Genv.add_global ge (a,ag)) a = Some (Genv.genv_next ge)).
-        unfold Genv.find_symbol, Genv.add_global; simpl. rewrite PTree.gss; auto.
-        forget (Genv.add_global ge (a,ag)) as ge1.
-        forget (Genv.genv_next ge) as N; clear ge H2.
-         assert (Zsucc N + Zlength dl > N).
-         rewrite Zlength_correct; unfold block in *; omega.
-         forget (Zsucc N + Zlength dl) as K.
-         clear - H1 H3 H2 H4.
-         revert ge1 K H2 H1 H3 H4; induction vl; simpl; intros. 
-        inversion2 H1 H4; omega.
-         apply (IHvl (Genv.add_global ge1 a0) K H2); auto.
-        unfold Genv.find_symbol, Genv.add_global in H4|-*; simpl in *.
-        rewrite PTree.gso; auto. 
-         apply IHdl; auto.
-        unfold Genv.find_symbol, Genv.add_global in H2|-*; simpl.
-                 rewrite PTree.gso; auto.
-Qed.
 
 Definition prog_var_block (rho: environ) (il: list ident) (b: block) : Prop :=
   Exists (fun id => match ge_of rho id with Some (Vptr b' _, _) => b'=b | _ => False end) il.
@@ -1394,125 +1180,6 @@ Proof.
  apply find_id_rev; auto.
 Qed.
 
-Lemma nth_error_rev:
-  forall T (vl: list T) (n: nat),
-   (n < length vl)%nat -> 
-  nth_error (rev vl) n = nth_error vl (length vl - n - 1).
-Proof.
- induction vl; simpl; intros. apply nth_error_nil.
- destruct (eq_dec n (length vl)).
- subst.
- pattern (length vl) at 1; rewrite <- rev_length.
- rewrite <- (plus_0_r (length (rev vl))).
- rewrite nth_error_app.
- case_eq (length vl); intros. simpl. auto.
- replace (S n - n - 1)%nat with O by omega.
- simpl; auto.
- rewrite nth_error_app1 by (rewrite rev_length; omega).
- rewrite IHvl by omega. clear IHvl.
- destruct n; destruct (length vl). congruence.
- simpl. replace (n-0)%nat with n by omega; auto.
- omegaContradiction.
- replace (S n1 - n - 1)%nat with (S (S n1 - S n - 1))%nat by omega.
- reflexivity.
-Qed.
-
-Lemma add_globals_hack:
-   forall vl gev,
-    list_norepet (map fst vl) ->
-    gev = Genv.add_globals (Genv.empty_genv fundef type) (rev vl) ->
-
-   (forall id b, 0 <= b-1 < Zlength vl ->
-                           (Genv.find_symbol gev id = Some b <->
-                            nth_error (map (@fst _ _) vl) (length vl - nat_of_Z b)  = Some id)).
-Proof. intros. subst.
-     apply iff_trans with (nth_error (map fst (rev vl)) (nat_of_Z (b - 1)) = Some id).
-Focus 2. rewrite map_rev; rewrite nth_error_rev.
-             replace (length (map fst vl) - nat_of_Z (b - 1) - 1)%nat 
-                        with (length vl - nat_of_Z b)%nat ; [intuition | ].
-  rewrite map_length.
-  transitivity (length vl - (nat_of_Z (b-1)+1))%nat; try omega.
-  f_equal.
-  change (nat_of_Z b = (nat_of_Z (b - 1) + nat_of_Z 1)%nat).
-  rewrite <- nat_of_Z_plus by omega.
-  f_equal. omega.
-  rewrite map_length.
-  rewrite Zlength_correct in H1.
-  forget (b-1) as i; forget (length vl) as n; clear - H1.
-  apply inj_lt_rev. rewrite nat_of_Z_max; auto. rewrite Zmax_spec. if_tac; omega.
-    rename H1 into Hb; revert H; induction vl; simpl; intros;
-       try rewrite Zlength_nil in *.
-      unfold Genv.find_symbol; simpl. rewrite PTree.gempty.
-     intuition. 
-       destruct a. inv H. rewrite Zlength_cons in Hb.
-       destruct (eq_dec (b-1) (Zlength vl)).
-        clear IHvl Hb. rewrite e. rewrite Zlength_correct. rewrite nat_of_Z_of_nat.
-        replace b with (1+ (Zlength vl)) by omega. clear e b.
-        rewrite <- Zlength_rev. rewrite <- rev_length.
-         replace (length (rev vl)) with (length (rev vl) + 0)%nat by omega.
-         rewrite map_app. rewrite <- map_length with (f:=@fst ident (globdef fundef type)).
-        rewrite nth_error_app. 
-        apply iff_trans with (i=id); [ | simpl; split; intro; subst; auto; inv H; auto].
-        rewrite In_rev in H2. rewrite <- map_rev in H2.
-       rewrite <- list_norepet_rev in H3. rewrite <- map_rev in H3.
-         forget (rev vl) as dl. 
-     apply find_symbol_add_globals; auto.   
-        spec IHvl ; [ omega |].
-      specialize (IHvl H3).
-      rewrite Genv.add_globals_app.
-      unfold Genv.add_globals at 1. simpl.
-        unfold Genv.find_symbol.
-       unfold Genv.add_global; simpl. 
-      destruct (eq_dec id i). subst i. rewrite PTree.gss.
-      rewrite Genv.genv_next_add_globals. rewrite <- Zlength_correct. simpl Genv.genv_next.
-     rewrite map_app.
-     rewrite In_rev in H2. rewrite <- map_rev in H2.
-     split; intro.
-     assert (b=1+Zlength (rev vl)) by congruence. clear H; subst b.
-
- elimtype False; clear - n; rewrite Zlength_rev in n; omega.
- f_equal.
- elimtype False.
-  assert (b-1 >= 0) by (clear - Hb; omega).
- pose proof (Coqlib.nat_of_Z_eq _ H0).
- clear - H1 H H2 n.
- rewrite Zlength_correct in n. apply n. clear n.
- rewrite <- H1.
- f_equal. clear - H H2.
- forget (nat_of_Z (b-1)) as j.
- replace (length vl) with (length (map fst (rev vl)))
-   by (rewrite map_length; rewrite rev_length; auto).
- forget (map fst (rev vl)) as al.
- revert al H2 H; clear; induction j; destruct al; simpl; intros; auto. inv H; intuition.
- elimtype False; clear - H; induction j; inv H; auto.
- f_equal. apply IHj; auto.
-
-    rewrite PTree.gso by auto. 
-  rewrite map_app.
-  destruct IHvl.
-  split; intro. apply H in H1. rewrite nth_error_app1; auto.
-  clear - n Hb. rewrite map_length. rewrite rev_length. rewrite Zlength_correct in Hb,n.
-  assert (b-1>=0) by omega.
- pose proof (Coqlib.nat_of_Z_eq _ H).
-  forget (nat_of_Z(b-1)) as j. rewrite <- H0 in *.
-   destruct Hb. clear - H2 n. omega. 
-  assert (nat_of_Z (b-1) < length (map (@fst _ _) (rev vl)))%nat.
-    clear - Hb n H1.
-  rewrite Zlength_correct in n. rewrite map_length; rewrite rev_length.
-  assert (nat_of_Z (b-1) <> length vl).
-  contradict n. rewrite <- n.
-  rewrite Coqlib.nat_of_Z_eq; auto. omega.
-  forget (nat_of_Z (b-1)) as j.
-  clear - H1 H.
-  assert (S (length vl) = length (map fst (rev vl) ++ map fst ((i, g) :: nil))).
-  simpl. rewrite app_length; rewrite map_length; rewrite rev_length; simpl; omega.
-  assert (j < S (length vl))%nat; [ | omega].
-  rewrite H0. forget (map fst (rev vl) ++ map fst ((i, g) :: nil)) as al.
-  clear - H1. revert al H1; induction j; destruct al; simpl in *; intros; inv H1; auto; try omega.
-  specialize (IHj _ H0); omega.
-  rewrite nth_error_app1 in H1 by auto.
-  apply H0 in H1. auto.
-Qed.
 
 Definition hackfun phi0 phi :=
   level phi0 = level phi /\
@@ -1739,7 +1406,7 @@ Proof.
  clear - z H0.
  unfold inflate_initial_mem; repeat rewrite resource_at_make_rmap.
  unfold inflate_initial_mem'.
- destruct (alloc_global_old _ _ _ _ H0 _ z). rewrite H; rewrite H1; auto. 
+ destruct (alloc_global_old _ _ _ _ H0 _ z) as [? [_ ?]]. rewrite H; rewrite H1; auto. 
  unfold upto_block. rewrite only_blocks_at. rewrite if_false by auto.
  unfold inflate_initial_mem; repeat rewrite resource_at_make_rmap;
    unfold inflate_initial_mem'.
